theories/logrel.v
@@ -1,0 +1,100 @@
+From iris.proofmode Require Import tactics.
+From iris.program_logic Require Export weakestpre.
+From iris.heap_lang Require Export lang.
+From iris.heap_lang Require Import proofmode notation.
+From iris.heap_lang.lib Require Import lock.
+From iris.heap_lang.lib Require Import spin_lock.
+From osiris Require Import typing auth_excl channel.
+From iris.algebra Require Import list auth excl.
+From iris.base_logic Require Import invariants auth saved_prop.
+Require Import FunctionalExtensionality.
+Import uPred.
+
+Section logrel.
+  Context `{!heapG Σ, !lockG Σ} (N : namespace).
+  Context `{!auth_exclG (list val) Σ}.
+  Context `{!auth_exclG stype Σ}.
+  
+  Record st_name := SessionType_name {
+    st_c_name : chan_name;
+    st_l_name : gname;
+    st_r_name : gname
+  }.
+
+  Definition stmapsto_frag γ (st : stype) s : iProp Σ :=
+    let γ :=
+        match s with
+        | Left  => st_l_name γ
+        | Right => st_r_name γ
+        end in
+    own γ (◯  to_auth_excl st)%I.
+
+  Definition stmapsto_full γ (st : stype) s : iProp Σ :=
+    let γ :=
+        match s with
+        | Left  => st_l_name γ
+        | Right => st_r_name γ
+        end in
+    own γ (● to_auth_excl st)%I.
+
+  Inductive st_eval : list val -> stype -> stype -> Prop :=
+    | st_eval_nil st : st_eval [] st (dual_stype st)
+    | st_eval_cons (P:val -> Prop) v vs st1 st2 :
+        P v -> st_eval vs st1 (st2 v) ->
+        st_eval (v::vs) st1 (TRecv P st2).
+  Hint Constructors st_eval.
+
+  Definition inv_st (γ :st_name) (c : val) : iProp Σ :=
+    (∃ l r stl str,
+      is_chan N (st_c_name γ) c l r ∗
+      stmapsto_full γ stl Left  ∗
+      stmapsto_full γ str Right ∗
+      ((⌜r = []⌝ ∗ ⌜st_eval r stl str⌝) ∨ 
+       (⌜l = []⌝ ∗ ⌜st_eval l stl str⌝)))%I.
+
+  Definition interp_st (γ : st_name) (st : stype) c s : iProp Σ :=
+    (stmapsto_frag γ st s ∗ inv N (inv_st γ c))%I.
+
+  Notation "⟦ ep : sτ ⟧{ γ }" :=
+  (interp_st γ sτ (ep.1) (ep.2))
+    (ep at level 99).
+
+  Lemma new_chan_vs st E c cγ :
+    is_chan N cγ c [] [] ={E}=∗
+      ∃ lγ rγ, 
+        let γ := SessionType_name cγ lγ rγ in
+        ⟦ (c,Left) : st ⟧{γ} ∗ ⟦ (c,Right) : (dual_stype st) ⟧{γ}.
+  Proof.
+    iIntros "Hc".
+    iMod (own_alloc (Auth (Excl' (to_auth_excl st)) (to_auth_excl st))) as (lγ) "Hlst"; first done.
+    iMod (own_alloc (Auth (Excl' (to_auth_excl (dual_stype st))) (to_auth_excl (dual_stype st)))) as (rγ) "Hrst"; first done.
+    rewrite (auth_both_op (to_auth_excl st)). 
+    rewrite (auth_both_op (to_auth_excl (dual_stype st))). 
+    rewrite own_op own_op.
+    iDestruct "Hlst" as "[Hlsta Hlstf]".
+    iDestruct "Hrst" as "[Hrsta Hrstf]".
+    pose (SessionType_name cγ lγ rγ) as stγ.
+    iMod (inv_alloc N _ (inv_st stγ c) with "[-Hlstf Hrstf]") as "#Hinv".
+    { iNext. rewrite /inv_st. eauto 10 with iFrame. }
+    eauto 10 with iFrame.
+  Qed.
+  
+  Lemma new_chan_st_spec st :
+    {{{ True }}}
+      new_chan #()
+    {{{ c γ, RET c; ⟦ (c,Left) : st ⟧{γ} ∗ ⟦ (c,Right) : dual_stype st ⟧{γ} }}}.
+  Proof.
+    iIntros (Φ _) "HΦ".
+    iApply (wp_fupd).
+    iApply (new_chan_spec)=> //.
+    iModIntro.
+    iIntros (c γ) "[Hc Hctx]".
+    iMod (new_chan_vs st ⊤ c γ with "[-HΦ]") as "H".
+    { rewrite /is_chan. eauto with iFrame. }
+    iDestruct "H" as (lγ rγ) "[Hl Hr]".
+    iApply "HΦ".
+    iModIntro.
+    iFrame.
+  Qed.      
+
+End logrel.
