theories/typing.v
@@ -1,0 +1,28 @@
+From iris.proofmode Require Import tactics.
+From iris.program_logic Require Export weakestpre.
+From iris.heap_lang Require Export lang.
+From stdpp Require Import gmap.
+From iris.base_logic Require Import invariants.
+Require Import FunctionalExtensionality.
+
+Section typing.
+
+  (* Sides *)
+  Inductive side : Set :=
+  | Left
+  | Right.
+
+  (* Session Types *)
+  Inductive stype :=
+  | TEnd
+  | TSend (P : heap_lang.val → Prop) (sτ : heap_lang.val → stype)
+  | TRecv (P : heap_lang.val → Prop) (sτ : heap_lang.val → stype).
+
+  Fixpoint dual_stype (sτ :stype) :=
+    match sτ with
+    | TEnd => TEnd
+    | TSend P sτ => TRecv P (λ v, dual_stype (sτ v))
+    | TRecv P sτ => TSend P (λ v, dual_stype (sτ v))
+    end.
+
+End typing.
